CollapsingTowers/TwoLvLBasic/Defs.lean
@@ -2,3 +2,4 @@ import CollapsingTowers.TwoLvLBasic.Syntax.Defs
 import CollapsingTowers.TwoLvLBasic.Utils.Defs
 import CollapsingTowers.TwoLvLBasic.Semantic.Defs
 import CollapsingTowers.TwoLvLBasic.SyntacticTyping.Defs
+import CollapsingTowers.TwoLvLBasic.Erasure.Defs
