CollapsingTowers/TwoLvLBasic/Erasure/Defs.lean
@@ -1,0 +1,2 @@
+import CollapsingTowers.TwoLvLBasic.Erasure.Env
+import CollapsingTowers.TwoLvLBasic.Erasure.Safety
