CollapsingTowers/TwoLvLBasic/Erasure/Env.lean
@@ -1,0 +1,52 @@
+import CollapsingTowers.TwoLvLBasic.SyntacticTyping.Defs
+
+@[simp]
+def ty.erase : Ty → Ty
+  | .nat => .nat
+  | .arrow τa τb _ => .arrow (erase τa) (erase τb) ∅
+  | .fragment τ => erase τ
+  | .rep τ => erase τ
+
+notation:max "‖" τ "‖𝜏" => ty.erase τ
+
+@[simp]
+def env.erase : TEnv → TEnv
+  | [] => []
+  | (τ, _) :: Γ => (‖τ‖𝜏, 𝟙) :: erase Γ
+
+notation:max "‖" Γ "‖𝛾" => env.erase Γ
+
+lemma ty.erase.wbt : ∀ 𝕊 τ, wbt 𝕊 ‖τ‖𝜏 :=
+  by
+  intros 𝕊 τ
+  induction τ
+  case nat => cases 𝕊 <;> simp
+  case arrow IH₀ IH₁ =>
+    cases 𝕊
+    case stat =>
+      constructor; apply IH₀; apply IH₁
+    case dyn =>
+      constructor; rfl
+      constructor; apply IH₀; apply IH₁
+  case fragment IH => apply IH
+  case rep IH => apply IH
+
+lemma env.erase.length : ∀ Γ, Γ.length = ‖Γ‖𝛾.length :=
+  by
+  intros Γ
+  induction Γ
+  case nil => rfl
+  case cons IH => simp; apply IH
+
+lemma env.erase.binds : ∀ x τ 𝕊 Γ, binds x (τ, 𝕊) Γ → binds x (‖τ‖𝜏, 𝟙) ‖Γ‖𝛾 :=
+  by
+  intros x τ 𝕊 Γ Hbinds
+  induction Γ
+  case nil => nomatch Hbinds
+  case cons tails IH =>
+    by_cases HEq : tails.length = x
+    . simp [if_pos HEq] at Hbinds
+      simp [← env.erase.length, if_pos HEq, Hbinds]
+    . simp [if_neg HEq] at Hbinds
+      simp [← env.erase.length, if_neg HEq]
+      apply IH; apply Hbinds
